@prefix : <https://schema.org/> .
@prefix rdf: <http://www.w3.org/1999/02/22-rdf-syntax-ns#> .
@prefix rdfs: <http://www.w3.org/2000/01/rdf-schema#> .
@prefix xml: <http://www.w3.org/XML/1998/namespace> .
@prefix xsd: <http://www.w3.org/2001/XMLSchema#> .

:Certification a rdfs:Class ;
	rdfs:label "Certification" ;
    :isPartOf <https://pending.schema.org> ;
    :source <https://github.com/schemaorg/schemaorg/issues/3230> ;	
    rdfs:comment """A Certification is an official and authoritative statement about a subject, for example a product, service, person, or organization. A certification is typically issued by an indendent certification body, for example a professional organization or government. It formally attests certain characteristics about the subject, for example Organizations can be ISO certified, Food products can be certified Organic or Vegan, a person can be a certified professional. There are certifications for many domains: regulatory, organizational, recycling, food, efficiency, educational, ecological, etc. A certification is a form of credential, as are accreditations and licenses. Same as GS1's [CertificationDetails](https://www.gs1.org/voc/CertificationDetails) type.""" ;
    rdfs:subClassOf :StructuredValue .

:auditDate a rdf:Property ;
    rdfs:label "auditDate" ;
    :domainIncludes :Certification ;
    :rangeIncludes :Date,
        :DateTime ;
    :source <https://github.com/schemaorg/schemaorg/issues/3230> ;
    rdfs:comment "Date when a certification was last audited. See also GS1 [certificationAuditDate](https://www.gs1.org/voc/certificationAuditDate)." .
	
:certificationRegistration a rdf:Property ;
    rdfs:label "certificationRegistration" ;
    :domainIncludes :Certification ;
    :isPartOf <https://pending.schema.org> ;
    :rangeIncludes :DefinedTerm,
        :Text ;
    :source <https://github.com/schemaorg/schemaorg/issues/3230> ;
    rdfs:comment "Registration key with an independent certification body. Typically this key can be used to consult and verify the certification. See also GS1 [certificationIdentification](https://www.gs1.org/voc/certificationIdentification)." .
		
:certificationType a rdf:Property ;
    rdfs:label "certificationType" ;
    :domainIncludes :Certification ;
    :isPartOf <https://pending.schema.org> ;
    :rangeIncludes :Thing;
    :source <https://github.com/schemaorg/schemaorg/issues/3230> ;
    rdfs:comment "Indicates the type of certification. See also GS1 [certificationType](https://www.gs1.org/voc/certificationType)." .

:CertificationStatusEnumeration a rdfs:Class ;
    rdfs:label "CertificationStatusEnumeration" ;
    :isPartOf <https://pending.schema.org> ;
    :source <https://github.com/schemaorg/schemaorg/issues/3230> ;
    rdfs:comment "Enumerates the different statuses of a Certification (Active and Inactive)." ;
    rdfs:subClassOf :Enumeration .	
	
:CertificationActive a :CertificationStatusEnumeration ;
    rdfs:label "CertificationActive" ;
    :isPartOf <https://pending.schema.org> ;
    :source <https://github.com/schemaorg/schemaorg/issues/3230> ;
    rdfs:comment "Specifies that a certification is active." .

:CertificationInactive a :CertificationStatusEnumeration ;
    rdfs:label "CertificationInactive" ;
    :isPartOf <https://pending.schema.org> ;
    :source <https://github.com/schemaorg/schemaorg/issues/3230> ;
    rdfs:comment "Specifies that a certification is inactive (no longer in effect)." .
	
:certificationStatus a rdf:Property ;
    rdfs:label "certificationStatus" ;
    :domainIncludes :Certification ;
    :rangeIncludes :CertificationStatusEnumeration;
    :source <https://github.com/schemaorg/schemaorg/issues/3230> ;
    rdfs:comment "Indicates the current status of a certification: active or inactive. See also GS1 [certificationStatus](https://www.gs1.org/voc/certificationStatus)." .
	
:hasCertification a rdf:Property ;
	rdfs:label "hasCertification" ;
	:domainIncludes :Product,
		 :Organization;
	:rangeIncludes :Certification;
	:source <https://github.com/schemaorg/schemaorg/issues/3230> ;
	rdfs:comment "Certification information about a product or organization." .




